Uppaal_Networks/AbsInt/Stack.thy
@@ -7,11 +7,11 @@ class absstack = bounded_semilattice_sup_bot + order_top
 locale AbsStack = AbsWord +
   fixes \<gamma>_stack :: "('b::absstack) \<Rightarrow> stack set" and
         push :: "'b \<Rightarrow> ('a::absword) \<Rightarrow> 'b" and
-        pop :: "'b \<Rightarrow> ('b * 'a)"
+        pop :: "'b \<Rightarrow> ('a * 'b)"
   assumes mono_gamma_stack: "a \<le> b \<Longrightarrow> \<gamma>_stack a \<le> \<gamma>_stack b"
   and gamma_Top[simp]: "\<gamma>_stack \<top> = \<top>"
   and push_correct: "c \<in> \<gamma>_stack b \<Longrightarrow> cx \<in> \<gamma>_word x \<Longrightarrow> (cx # c) \<in> \<gamma>_stack (push b x)"
-  and pop_stack_correct:  "(cx # c) \<in> \<gamma>_stack b \<Longrightarrow> c \<in> \<gamma>_stack (fst (pop b))"
-  and pop_return_correct: "(cx # c) \<in> \<gamma>_stack b \<Longrightarrow> cx \<in> \<gamma>_word (snd (pop b))"
+  and pop_stack_correct:  "(cx # c) \<in> \<gamma>_stack b \<Longrightarrow> c \<in> \<gamma>_stack (snd (pop b))"
+  and pop_return_correct: "(cx # c) \<in> \<gamma>_stack b \<Longrightarrow> cx \<in> \<gamma>_word (fst (pop b))"
 
 end
